\section{Arrows in Haskell}

\frame{\tableofcontents[currentsection]}

\begin{frame}
    \begin{itemize}
        \item Monads take types to computations with result type
        \item No parametrically structured input requirements
        \item \emph{Arrows} as generalizations of computation $X$ to $Y$
        \item Two-parametric, $(X, Y) \mapsto A(X, Y)$
        \item Uniform access to structure on computation input
    \end{itemize}
\end{frame}

\begin{frame}[fragile]
    \begin{definition}[\texttt{Arrow} type class]
        \begin{code}
class Arrow a where
  -- Embed pure computation
  arr   :: (b -> c) -> a b c
  -- Precomposition
  (>>>) :: a b c -> a c d -> a b d
  -- Left-side application
  first :: a b c -> a (b, d) (c, d)

  -- Right-side application (definable)
  (second) :: a b c -> a (b, d) (c, d)
  second f = arr swap >>> first f >>> arr swap

  -- Non-commutative product (definable)
  (***) :: a b c -> a b' c' -> a (b, b') (c, c')
  f *** g = first f >>> second g
        \end{code}
    \end{definition}
\end{frame}

\begin{frame}[fragile]
\begin{definition}[Arrow Laws]
\begin{code}[numbers=left]
              (a >>> b) >>> c == a >>> (b >>> c)
                  arr (g . f) == arr f >>> arr g
                  arr id >>> a == a
                             a == a >>> arr id
           first a >>> arr fst == arr fst >>> a
    first a >>> arr (id *** f) == arr (id *** f) >>> first a
 first (first a) >>> arr assoc == arr assoc >>> first a
                 first (arr f) == arr (f *** id)
               first (a >>> b) == first a >>> first b
\end{code}
Here \verb|assoc| flips tuples \verb|((a,b),c)| to \verb|(a,(b,c))|.
\end{definition}
\end{frame}

\begin{frame}[fragile]
\begin{example}[Pure Functions as Arrows]
\begin{code}
instance Arrow (->) where
    arr f   = f
    f >>> g = g . f
    first f = \symbol{92}(x, y) -> (f x, y)
\end{code}
\end{example}
\end{frame}

\begin{frame}[fragile]
\begin{example}[State Arrows]
\begin{code}
-- Define type
newtype State s x y = ST ((s, x) -> (s, y))

instance Arrow (State s) where
    arr f         = ST (id *** f)
    ST f >>> ST g = ST (g . f)
    first (ST f)  = ST (assoc . (f *** id) . unassoc)

-- A state changing arrow
count :: State Int x y
count = ST ((+1) *** id)
\end{code}
\end{example}
\end{frame}
